lift tactic: work-in-progress

src/Pipit.Sugar.Shallow.Tactics.Lift.fst
@@ -1,12 +1,6 @@
 (* box/lift transform *)
 module Pipit.Sugar.Shallow.Tactics.Lift
 
-// module PPT = Pipit.Prim.Table
-// module PPS = Pipit.Prim.Shallow
-// module SB  = Pipit.Sugar.Base
-// module SSB = Pipit.Sugar.Shallow.Base
-
-module RefV1 = FStar.Reflection.V1
 module Ref = FStar.Reflection.V2
 module Tac = FStar.Tactics.V2
 
@@ -14,20 +8,23 @@ module List = FStar.List.Tot
 
 // #push-options "--print_implicits --print_full_names --ugly"
 
-type stream (a: eqtype) = nat -> a
+assume new type stream (a: eqtype)
 
-[@@"opaque_to_smt"]
-let rec'
-  (f: stream 'a -> stream 'a): stream 'a =
-  (fun ix ->
-    f (admit ()) ix)
+assume new type stream_app (a: Type)
 
-[@@"opaque_to_smt"]
-let (let^) (f: stream 'a) (g: stream 'a -> stream 'b): stream 'b =
-    g f
+assume val liftP'prim (#ft: Type) (f: ft): stream_app ft
 
-[@@"opaque_to_smt"]
-let return (#a: eqtype) (x: a): stream a = (fun ix -> x)
+assume val liftP'apply (#a: eqtype) (#ft: Type) (f: stream_app (a -> ft)) (ea: stream a): stream_app ft
+
+assume val liftP'close (#a: eqtype) (ea: stream_app a): stream a
+
+assume val rec' (#a: eqtype) (f: stream a -> stream a): stream a
+
+assume val (let^) (#a #b: eqtype) (f: stream a) (g: stream a -> stream b): stream b
+
+assume val return (#a: eqtype) (x: a): stream a
+
+assume val fby (#a: eqtype) (x: a) (xs: stream a): stream a
 
 unfold
 let nolift (#a: eqtype) (x: a): a = x
@@ -53,12 +50,12 @@ let env_get_mode (b: Tac.namedv) (e: env): Tac.Tac mode =
   | None -> Tac.fail ("no such binder: b" ^ Tac.namedv_to_string b)
   | Some (_, m) -> m
 
-let stream_ty_unify_get_elt (e: env) (ty: Tac.term): Tac.Tac Tac.term =
-  let uvar = Tac.uvar_env e.tac_env (Some (`eqtype)) in
-  let expect = (`stream (`#uvar)) in
-  if Tac.unify_env e.tac_env ty expect
-  then uvar
-  else Tac.fail ("expected stream type; got type " ^ Tac.term_to_string ty)
+// let stream_ty_unify_get_elt (e: env) (ty: Tac.term): Tac.Tac Tac.term =
+//   let uvar = Tac.uvar_env e.tac_env (Some (`eqtype)) in
+//   let expect = (`stream (`#uvar)) in
+//   if Tac.unify_env e.tac_env ty expect
+//   then uvar
+//   else Tac.fail ("expected stream type; got type " ^ Tac.term_to_string ty)
 
 
 let mode_of_ty (e: env) (ty: Tac.term): Tac.Tac (mode & Tac.term) =
@@ -92,17 +89,9 @@ let mode_join (m1 m2: mode): mode = match m1, m2 with
   | _, Stream -> Stream
   | Pure, Pure -> Pure
 
-let mode_opt_join (m1 m2: option mode): option mode = match m1, m2 with
-  | None, _ -> m2
-  | _, None -> m1
-  | Some Stream, _ -> Some Stream
-  | _, Some Stream -> Some Stream
-  | Some Pure, Some Pure -> Some Pure
-
 let modes_of_arr (e: env) (ty: Tac.term): Tac.Tac (option (list mode & mode)) =
   match Tac.collect_arr ty with
   | args, Tac.C_Total res ->
-    // TODO: avoid unification?
     let margs = Tac.map (mode_of_ty' e) args in
     let mres = mode_of_ty' e res in
     if List.existsb (fun m -> m = Stream) (mres::margs)
@@ -136,8 +125,9 @@ let rec descend (e: env) (t: Tac.term): Tac.Tac (mode & Tac.term) =
   | Tac.Tv_Var (v: Tac.namedv) ->
     (env_get_mode v e, t)
   | Tac.Tv_BVar (v: Tac.bv) ->
-    Tac.fail ("Lift.descend: unexpected bvar? " ^ Tac.term_to_string t)
+    Tac.fail ("Lift.descend: unexpected bvar; expected named variables only " ^ Tac.term_to_string t)
   | Tac.Tv_FVar (v: Tac.fv) ->
+    // DISALLOW: ensure no unapplied functions?
     (mode_of_ty' e (Tac.tc e.tac_env t), t)
   | Tac.Tv_Const (vc: Tac.vconst) ->
     (Pure, t)
@@ -148,11 +138,13 @@ let rec descend (e: env) (t: Tac.term): Tac.Tac (mode & Tac.term) =
       | [] -> hd
     in
     let rec mk_lift_apps hd args: Tac.Tac Tac.term = match args with
-    //TODO DO LIFT
-      | (mm,arg,aqual)::args -> mk_lift_apps (Tac.pack (Tac.Tv_App hd (arg,aqual))) args
+      | (mm,arg,aqual)::args ->
+        // TODO aqual: handle implicit parameters
+        // CHECK: ensure fully applied? partial-applications will fail as no stream instance
+        let (mm, arg) = mode_cast e Stream (Tac.pack Tac.Tv_Unknown) (mm, arg) in
+        mk_lift_apps (`liftP'apply (`#hd) (`#arg)) args
       | [] ->
-        debug_print "TODO:LIFT!";
-      hd
+        hd
     in
     let rec go_lifts hd args m collect: Tac.Tac (mode & Tac.term) = match args with
       | (arg,aqual)::args ->
@@ -161,18 +153,22 @@ let rec descend (e: env) (t: Tac.term): Tac.Tac (mode & Tac.term) =
       | [] ->
         (match m with
         | Pure -> (Pure, mk_pure_apps hd (List.rev collect))
-        | Stream -> (Stream, mk_lift_apps hd (List.rev collect)))
+        | Stream ->
+          let hd = (`liftP'prim (`#hd)) in
+          (Stream, `liftP'close (`#(mk_lift_apps hd (List.rev collect)))))
     in
     let rec mk_apps hd modes args: Tac.Tac Tac.term = match modes, args with
       | mx::modes, (arg,aqual)::args ->
         let (ma, arg) = descend e arg in
         // XXX: is tc here necessary?
-        let (ma, arg) = mode_cast e mx (Tac.tc e.tac_env arg) (ma, arg) in
+        let (ma, arg) = mode_cast e mx (Tac.pack Tac.Tv_Unknown) (ma, arg) in
+        // let (ma, arg) = mode_cast e mx (Tac.tc e.tac_env arg) (ma, arg) in
         mk_apps (Tac.pack (Tac.Tv_App hd (arg, aqual))) modes args
       | _, _ -> hd
     in
     let rec go_apps hd args: Tac.Tac (mode & Tac.term) = match Tac.inspect hd with
       | Tac.Tv_FVar (v: Tac.fv) ->
+        // XXX: this fails for record accessors, and lookup_typ returns None
         let ty = Tac.tc e.tac_env hd in
         (match modes_of_arr e ty with
         | None -> go_lifts hd args Pure []
@@ -186,11 +182,11 @@ let rec descend (e: env) (t: Tac.term): Tac.Tac (mode & Tac.term) =
     in
     go_apps hd [(arg, aqual)]
   | Tac.Tv_Abs bv tm ->
+    // CHECK: only allow abs at top level?
     debug_print ("Abs: descend with " ^ Tac.term_to_string bv.sort);
     let (mt, tm) = descend (env_push bv (mode_of_ty' e bv.sort) e) tm in
     (mt, Tac.pack (Tac.Tv_Abs bv tm))
 
-  | Tac.Tv_Uvar _ _ -> (Pure, t)
 
   | Tac.Tv_Let true attrs b def body ->
     debug_print ("letrec: binder type: " ^ Tac.term_to_string (b.sort));
@@ -232,8 +228,28 @@ let rec descend (e: env) (t: Tac.term): Tac.Tac (mode & Tac.term) =
     (mode_join md mb, lett)
 
   | Tac.Tv_Match scrut ret brs ->
-    //TODO: only lift matches with no binders to start with
-    (Pure, t)
+    let (ms, scrut) = descend e scrut in
+    (match ms with
+    | Pure ->
+      let rec go_pure brs: Tac.Tac (mode & list Tac.branch) = match brs with
+        | [] -> (Pure, [])
+        | (pat,tm) :: brs ->
+          let (m,brs) = go_pure brs in
+          let (mt,tm) = descend e tm in
+          (mode_join m mt, (pat,tm) :: brs)
+      in
+      let (mb, brs) = go_pure brs in
+      (mb, Tac.pack (Tac.Tv_Match scrut ret brs))
+    | Stream ->
+      let rec go_stream brs: Tac.Tac (mode & list Tac.branch) = match brs with
+        | [] -> (Pure, [])
+        | (pat,tm) :: brs ->
+          let (m,brs) = go_stream brs in
+          let (mt,tm) = descend e tm in
+          (mode_join m mt, (pat,tm) :: brs)
+      in
+      let (mb, brs) = go_stream brs in
+      (mb, Tac.pack (Tac.Tv_Match scrut ret brs)))
 
   | Tac.Tv_AscribedT (tm: Tac.term) (ty: Tac.term) tac use_eq ->
     debug_print ("AscribedT: " ^ Tac.term_to_string ty);
@@ -252,6 +268,7 @@ let rec descend (e: env) (t: Tac.term): Tac.Tac (mode & Tac.term) =
     | _ -> Tac.fail "unsupported: type ascriptions on effects")
 
   // Type stuff: leave alone
+  | Tac.Tv_Uvar _ _ -> (Pure, t)
   | Tac.Tv_UInst (v: Tac.fv) (us: Tac.universes) -> (Pure, t)
   | Tac.Tv_Arrow  bv c -> (Pure, t)
   | Tac.Tv_Type   u    -> (Pure, t)
@@ -274,27 +291,59 @@ let tac_lift (t: Tac.term): Tac.Tac Tac.term =
 let fst (#a #b: eqtype): (a & b) -> a = fst
 
 
-
+// do not support local function bindings yet
 // [@@Tac.preprocess_with tac_lift]
-// let pp_letrecfun (x: int): int =
+// let eg_letrecfun (x: int): int =
 //   let rec count x = if x > 0 then count (x - 1) else 0 in
 //   count 0
 
 [@@Tac.preprocess_with tac_lift]
-let pp_letrec (x: stream int): stream int =
-  let rec count: stream int = count in // if count > 0 then count else 0 in
+let eg_letrec (x: stream int): stream int =
+  let rec count = 0 `fby` count + 1 in
   let y = (0 <: stream int) in
   // let z: stream int = 0 in
   // let rec count (i: int): int = count i in
-  1 + y + count
+  (1 + y) + count
+
+[@@Tac.preprocess_with tac_lift]
+let eg_pairs (x: stream int): stream int =
+  0 `fby` fst (x, x)
+
+
+type ctor = | Ctor: x: int -> y: int -> ctor
+[@@Tac.preprocess_with tac_lift]
+let eg_ctor (add: stream int): stream ctor =
+  let rec rcd =
+    let x = 0 `fby` Ctor?.x rcd + add in
+    let y = 0 `fby` Ctor?.y rcd - add in
+    Ctor x y
+  in
+  rcd
+
+[@@Tac.preprocess_with tac_lift]
+let eg_pairsrec (add: stream int): stream (int & int) =
+  let rec xy =
+    // let (x,y) = xy in
+    let x = 0 `fby` fst xy + add in
+    let y = 0 `fby` snd xy - add in
+    (x, y)
+  in
+  xy
+
+// fails: cannot typecheck record accessors?
+// type record = { x: int; y: int; }
+// [@@Tac.preprocess_with tac_lift]
+// let eg_record (add: stream int): stream int =
+//   let rec rcd =
+//     let x = 0 `fby` rcd.x + add in
+//     let y = 0 `fby` rcd.y - add in
+//     {x; y}
+//   in
+//   rcd
+
 
 // [@@Tac.preprocess_with tac_lift]
-// let pp_pairs (x: stream int): stream (int & int) =
-//   (x, x)
-
-
-// [@@Tac.preprocess_with tac_lift]
-// let pp_let (x: stream int): stream int =
+// let eg_let (x: stream int): stream int =
   // let y: stream (int & int) = (x + 1, x - 1)
   // in
   // let z: stream int = fst y in
@@ -303,22 +352,22 @@ let pp_letrec (x: stream int): stream int =
   // z
 
 // [@@Tac.preprocess_with lift]
-// let pp_letop (x: int): int =
+// let eg_letop (x: int): int =
 //   let^ y: int = x + 1
 //   in y
 
 // [@@Tac.preprocess_with lift]
-// let pp_letrec_fun (x: int): int =
+// let eg_letrec_fun (x: int): int =
 //   let rec a z = if z >= 0 then x else a (z - 1)
 //   in a x
 
 // [@@Tac.preprocess_with lift]
-// let pp_letrec_strm (x: int): int =
+// let eg_letrec_strm (x: int): int =
 //   let rec a = x + a
 //   in a
 
 // [@@Tac.preprocess_with lift]
-// let pp_letrec_mut (x: int): int =
+// let eg_letrec_mut (x: int): int =
 //   let rec a = x + b
 //       and b = x - a
 //   in a
